Trestle/Data.lean
@@ -1,4 +1,5 @@
 import Trestle.Data.Cnf
 import Trestle.Data.HashAssn
 import Trestle.Data.ICnf
+import Trestle.Data.RichCnf
 import Trestle.Data.Literal
