Trestle/Data/Cnf/Basic.lean
@@ -1,0 +1,291 @@
+/-
+Copyright (c) 2025 The Trestle Contributors.
+Released under the Apache License v2.0; see LICENSE for full text.
+-/
+
+import Trestle.Data.Cnf.Defs
+import Trestle.Data.LitVar.Basic
+import Trestle.Model.PropVars
+
+namespace Trestle
+
+open Model
+
+namespace Clause
+
+variable {L : Type u} {ν : Type v} [LitVar L ν]
+
+def toPropFun (C : Clause L) : PropFun ν :=
+  .any (Multiset.ofList C.toList |>.map LitVar.toPropFun)
+
+instance instCoeToPropFun : CoeHead (Clause L) (PropFun ν) := ⟨toPropFun⟩
+
+theorem mem_semVars_toPropFun [DecidableEq ν] (x : ν) (C : Clause L)
+  : x ∈ C.toPropFun.semVars → ∃ l, l ∈ C ∧ LitVar.toVar l = x := by
+  intro h
+  rcases C with ⟨data⟩
+  have ⟨τ,hpos,hneg⟩ := (PropFun.mem_semVars _ _).mp h; clear h
+  simp_all [toPropFun, Array.mem_def]
+  rcases hpos with ⟨l,hl,h⟩
+  have := (PropFun.mem_semVars _ _).mpr ⟨τ,h,hneg l hl⟩; clear hneg h
+  aesop
+
+open PropFun
+
+theorem satisfies_iff {τ : PropAssignment ν} {C : Clause L} :
+    τ ⊨ C.toPropFun ↔ ∃ l ∈ C, τ ⊨ LitVar.toPropFun l := by
+  simp_rw [toPropFun, Array.mem_def]
+  simp
+
+theorem tautology_iff [DecidableEq ν] [LawfulLitVar L ν] (C : Clause L) :
+    C.toPropFun = ⊤ ↔ ∃ l₁ ∈ C, ∃ l₂ ∈ C, l₁ = -l₂ := by
+  constructor
+  · intro h
+    rcases C with ⟨lits⟩
+    simp_all [toPropFun, Array.mem_def]
+    induction lits with
+    | nil => rw [PropFun.ext_iff] at h; simp [Array.mem_def] at h
+    | cons hd tl ih =>
+    classical
+    refine if hr : any _ = ⊤ then have := ih hr; ?_ else ?_
+    · aesop
+    · clear ih
+      rw [PropFun.ext_iff] at hr h
+      simp at hr h
+      rcases hr with ⟨τ,hr⟩
+      replace h := h (τ.set (LitVar.toVar hd) (!LitVar.polarity hd))
+      simp [LitVar.satisfies_iff, Bool.not_ne_self] at h
+      rcases h with ⟨hd',hd'_mem,h⟩
+      · replace hr := hr hd' hd'_mem
+        simp [LitVar.satisfies_iff, PropAssignment.set] at hr h
+        use hd, (List.mem_cons_self _ _), hd', (List.mem_cons_of_mem _ hd'_mem)
+        split at h
+        · ext
+          · rw [LawfulLitVar.toVar_negate]; symm; assumption
+          · rw [LawfulLitVar.polarity_negate]; exact Bool.not_eq_eq_eq_not.mp h
+        · exact absurd h hr
+  · rintro ⟨_,hl1,l,hl2,rfl⟩
+    ext τ; simp [satisfies_iff]
+    by_cases τ ⊨ LitVar.toPropFun l <;> aesop
+
+@[simp] theorem toPropFun_or (c1 c2 : Clause L)
+  : (c1.or c2).toPropFun = c1.toPropFun ⊔ c2.toPropFun := by
+  ext τ
+  simp [or, satisfies_iff]
+  apply Iff.intro
+  · rintro ⟨l,h1,h2⟩
+    cases h1
+    · refine Or.inl ⟨l,?_⟩
+      simp [*]
+    · refine Or.inr ⟨l,?_⟩
+      simp [*]
+  · rintro (⟨l,h1,h2⟩|⟨l,h1,h2⟩)
+    · refine ⟨l,?_⟩
+      simp [*]
+    · refine ⟨l,?_⟩
+      simp [*]
+
+@[simp] theorem toPropFun_map [LitVar L' ν'] [LawfulLitVar L' ν'] (f : ν → ν') (c : Clause L)
+  : (c.map L' f).toPropFun = c.toPropFun.map f
+  := by
+  ext τ
+  simp [map, satisfies_iff]
+
+@[simp] theorem toPropFun_empty : Clause.toPropFun (#[] : Clause L) = ⊥ := rfl
+@[simp] theorem toPropFun_nil : Clause.toPropFun ({ toList := [] } : Clause L) = ⊥ := rfl
+
+@[simp]
+theorem toPropFun_cons (l : L) (C : List L)
+  : Clause.toPropFun { toList := l :: C } = LitVar.toPropFun l ⊔ Clause.toPropFun { toList := C } := rfl
+
+end Clause
+
+/-! ### CNF -/
+
+namespace Cnf
+
+variable {L : Type u} {ν : Type v} [LitVar L ν]
+
+def toPropFun (φ : Cnf L) : PropFun ν :=
+  .all (φ.toList.map Clause.toPropFun)
+
+theorem semVars_toPropFun [DecidableEq ν] (F : Cnf L)
+  : v ∈ (toPropFun F).semVars → ∃ C, C ∈ F ∧ ∃ l, l ∈ C ∧ LitVar.toVar l = v := by
+  rcases F with ⟨F⟩; simp_rw [Array.mem_def]; simp [toPropFun, PropFun.all]
+  induction F <;> simp
+  next hd tl ih =>
+  intro hv
+  have := PropFun.semVars_conj _ _ hv
+  simp at this
+  rcases this with (h|h)
+  · have := Clause.mem_semVars_toPropFun _ _ h
+    simp_rw [Array.mem_def] at this
+    aesop
+  · have := ih h
+    simp_rw [Array.mem_def] at *
+    simp_all
+
+instance : CoeHead (Cnf L) (PropFun ν) := ⟨toPropFun⟩
+
+theorem mem_semVars_toPropFun [DecidableEq ν] (x : ν) (F : Cnf L)
+  : x ∈ F.toPropFun.semVars → ∃ C, C ∈ F ∧ x ∈ C.toPropFun.semVars := by
+  intro h
+  rcases F with ⟨data⟩
+  simp [Array.mem_def]
+  induction data <;> simp_all [toPropFun, PropFun.all]
+  replace h := PropFun.semVars_conj _ _ h
+  aesop
+
+open PropFun
+
+theorem satisfies_iff {τ : PropAssignment ν} {φ : Cnf L} :
+    τ ⊨ φ.toPropFun ↔ ∀ C ∈ φ, τ ⊨ C.toPropFun := by
+  rw [toPropFun]
+  rcases φ with ⟨φ⟩
+  induction φ <;> simp_all [Array.mem_def]
+
+@[simp]
+theorem toPropFun_addClause (C : Clause L) (f : Cnf L)
+    : (f.addClause C).toPropFun = f.toPropFun ⊓ C.toPropFun := by
+  have ⟨C⟩ := C
+  have ⟨f⟩ := f
+  ext τ
+  simp [satisfies_iff, addClause]
+  constructor
+  · intro h
+    constructor
+    · intro C' hC'
+      exact h C' (Or.inl hC')
+    · exact h _ (Or.inr rfl)
+  · rintro ⟨hF, hC⟩ C' (hC' | rfl)
+    · exact hF _ hC'
+    · exact hC
+
+@[simp]
+theorem toPropFun_and (f1 f2 : Cnf L)
+    : (f1.and f2).toPropFun = f1.toPropFun ⊓ f2.toPropFun := by
+  have ⟨f1⟩ := f1
+  have ⟨f2⟩ := f2
+  ext τ
+  simp [satisfies_iff, and]
+  constructor
+  · intro h
+    constructor
+    <;> intro C hC
+    · exact h C (Or.inl hC)
+    · exact h C (Or.inr hC)
+  · rintro ⟨h₁, h₂⟩ C (hC | hC)
+    · exact h₁ _ hC
+    · exact h₂ _ hC
+
+@[simp]
+theorem toPropFun_not (c : Clause L) [LawfulLitVar L ν]
+    : (not c).toPropFun = (c.toPropFun)ᶜ := by
+  have ⟨c⟩ := c
+  ext τ
+  simp [not, satisfies_iff, Clause.satisfies_iff, LitVar.satisfies_iff]
+  constructor
+  · intro h l h_mem hl
+    simp [h _ h_mem] at hl
+  · intro h l h_mem
+    exact Bool.eq_not.mpr (h l h_mem)
+
+@[simp]
+theorem toPropFun_any (ls : Array L)
+    : (any ls).toPropFun = .any (ls.toList.map LitVar.toPropFun) := by
+  have ⟨ls⟩ := ls
+  ext τ
+  simp [any, toPropFun, Clause.toPropFun]
+
+@[simp]
+theorem toPropFun_all (ls : Array L)
+    : (all ls).toPropFun = .all (ls.toList.map LitVar.toPropFun) := by
+  have ⟨ls⟩ := ls
+  ext τ
+  simp [satisfies_iff, Clause.satisfies_iff, LitVar.satisfies_iff, all]
+
+/-! #### Satisfiability -/
+
+abbrev Sat (f : Cnf L) : Prop := f.toPropFun.Sat
+
+end Cnf
+
+namespace Cube
+
+variable [LitVar L ν]
+
+def toPropFun (C : Cube L) : PropFun ν :=
+  .all (Multiset.ofList C.toList |>.map LitVar.toPropFun)
+
+instance : CoeHead (Cube L) (PropFun ν) := ⟨toPropFun⟩
+
+theorem mem_semVars_toPropFun [DecidableEq ν] (x : ν) (C : Cube L)
+  : x ∈ C.toPropFun.semVars → ∃ l, l ∈ C.toArray ∧ LitVar.toVar l = x := by
+  intro h
+  rcases C with ⟨data⟩
+  have ⟨τ,hpos,hneg⟩ := (PropFun.mem_semVars _ _).mp h; clear h
+  simp_all [toPropFun, Array.mem_def]
+  rcases hneg with ⟨l,hl,h⟩
+  have := (PropFun.mem_semVars _ _).mpr ⟨τ,hpos l hl,h⟩; clear hpos h
+  aesop
+
+open PropFun
+
+theorem satisfies_iff {τ : PropAssignment ν} {C : Cube L} :
+    τ ⊨ C.toPropFun ↔ ∀ l ∈ C.toArray, τ ⊨ LitVar.toPropFun l := by
+  simp_rw [toPropFun, Array.mem_def]
+  simp
+
+theorem empty_iff [DecidableEq ν] [LawfulLitVar L ν] (C : Cube L) :
+    C.toPropFun = ⊥ ↔ ∃ l₁ ∈ C.toArray, ∃ l₂ ∈ C.toArray, l₁ = -l₂ := by
+  constructor
+  · intro h
+    rcases C with ⟨lits⟩
+    simp_all [toPropFun, Array.mem_def]
+    induction lits with
+    | nil => rw [PropFun.ext_iff] at h; simp [Array.mem_def] at h
+    | cons hd tl ih =>
+    classical
+    refine if hr : all _ = ⊥ then have := ih hr; ?_ else ?_
+    · aesop
+    · clear ih
+      rw [PropFun.ext_iff] at hr h
+      simp at hr h
+      rcases hr with ⟨τ,hr⟩
+      replace h := h (τ.set (LitVar.toVar hd) (LitVar.polarity hd)) (by
+        simp [LitVar.satisfies_iff])
+      simp at h
+      rcases h with ⟨hd',hd'_mem,h⟩
+      replace hr := hr hd' hd'_mem
+      simp [LitVar.satisfies_iff, PropAssignment.set] at hr h
+      split at h
+      · use hd, (List.mem_cons_self _ _), hd', (List.mem_cons_of_mem _ hd'_mem)
+        ext
+        · rw [LawfulLitVar.toVar_negate]; symm; assumption
+        · rw [LawfulLitVar.polarity_negate, Bool.eq_not]; assumption
+      · exact absurd hr h
+  · rintro ⟨_,hl1,l,hl2,rfl⟩
+    ext τ; simp [satisfies_iff]
+    by_cases τ ⊨ LitVar.toPropFun l <;> aesop
+
+@[simp] theorem toPropFun_and (c1 c2 : Cube L)
+  : (c1.and c2).toPropFun = c1.toPropFun ⊓ c2.toPropFun := by
+  ext τ
+  simp [and, satisfies_iff]
+  apply Iff.intro
+  · rintro h
+    constructor
+    · aesop
+    · aesop
+  · rintro h l (l_mem|l_mem) <;>
+      aesop
+
+@[simp] theorem toPropFun_map [LitVar L' ν'] [LawfulLitVar L' ν'] (f : ν → ν') (c : Cube L)
+  : (c.map L' f).toPropFun = c.toPropFun.map f
+  := by
+  ext τ
+  simp [map, satisfies_iff]
+
+end Cube
+
+end Trestle
