Trestle/Data/Cnf/Defs.lean
@@ -1,0 +1,93 @@
+import Trestle.Data.LitVar.Defs
+
+import Batteries.Data.List.Basic
+
+namespace Trestle
+
+/-- A disjunction of literals -/
+abbrev Clause (L : Type u) := Array L
+
+/-- A conjunction of clauses -/
+abbrev Cnf (L : Type u) := Array (Clause L)
+
+/-- A conjunction of literals.
+The implementation is identical to clauses,
+but the interpretation is different.
+-/
+def Cube (L : Type u) := Array L
+
+namespace Clause
+
+instance instToString [ToString L] : ToString (Clause L) where
+  toString C := s!"({String.intercalate " ∨ " (C.map toString).toList})"
+
+variable {L : Type u} {ν : Type v} [LitVar L ν]
+
+def or (c1 c2 : Clause L) : Clause L :=
+  c1 ++ c2
+
+def negate (c : Clause L) : Cube L :=
+  Array.map (-·) c
+
+nonrec def map (L') [LitVar L' ν'] (f : ν → ν') (c : Clause L) : Clause L' :=
+  c.map (LitVar.map f)
+
+end Clause
+
+namespace Cnf
+
+instance instToString [ToString L] : ToString (Cnf L) where
+  toString C := s!"{String.intercalate " ∧ " (C.map toString).toList}"
+
+variable {L : Type u} {ν : Type v} [LitVar L ν]
+
+def addClause (f : Cnf L) (C : Clause L) : Cnf L := f.push C
+
+def and (f1 f2 : Cnf L) : Cnf L := f1 ++ f2
+
+def not (c : Clause L) : Cnf L :=
+  Array.map (fun l => #[-l]) c
+
+def any (ls : Array L) : Cnf L := #[ls]
+
+def all (ls : Array L) : Cnf L :=
+  Array.map (fun l => #[l]) ls
+
+end Cnf
+
+
+namespace Cube
+
+instance [ToString L] : ToString (Cube L) where
+  toString C := s!"({String.intercalate " ∧ " (C.map toString).toList})"
+
+variable {L : Type u} {ν : Type v} [LitVar L ν]
+
+abbrev toArray (c : Cube L) : Array L := c
+
+instance : CoeHead (Cube L) (Array L) := ⟨toArray⟩
+
+def and (c1 c2 : Cube L) : Cube L :=
+  c1.toArray ++ c2.toArray
+
+nonrec def map (L') [LitVar L' ν'] (f : ν → ν') (c : Cube L) : Cube L' :=
+  c.map (LitVar.map f)
+
+def negate (c : Cube L) : Clause L :=
+  Array.map (- ·) c
+
+end Cube
+
+abbrev Cubing (L) := List (Cube L)
+
+namespace Cubing
+
+def unit : Cubing L := [#[]]
+
+def prod (c1 c2 : Cubing L) : Cubing L :=
+  List.product c1 c2
+  |>.map fun (a,b) => a.and b
+
+end Cubing
+
+end Trestle
