Trestle/Data/ICnf/Defs.lean
@@ -1,0 +1,282 @@
+/-
+Copyright (c) 2025 The Trestle Contributors.
+Released under the Apache License v2.0; see LICENSE for full text.
+-/
+
+import Trestle.Data.LitVar.Defs
+import Trestle.Data.Cnf.Defs
+import Trestle.Upstream.ToStd
+
+/-
+
+Implementations of DIMACS literals, variables, and formulas.
+
+-/
+
+namespace Trestle
+
+-- TODO: We could add an implementation type that uses `UInt64` or `USize` instead,
+--       since almost all CNF instances will use "small" variable names.
+
+/--
+  The implementation type of DIMACS variables (hence the "I" in `IVar`).
+
+  In DIMACS, variables are represented by strictly positive integers.
+  We attach the positivity-hypothesis as a subtype here.
+
+  This type is the exact same as the one for `PNat` in Mathlib
+  (see [Data.PNat.Defs.lean](https://github.com/leanprover-community/mathlib4/blob/master/Mathlib/Data/PNat/Defs.lean)).
+  We redefine it here to avoid the dependency on Mathlib,
+  and also in case we want to change the backing type to `UInt64` in the future.
+-/
+def IVar := { n : Nat // 0 < n }
+  deriving DecidableEq, Repr
+
+/--
+  The implementation type of DIMACS literals (hence the "I" in `ILit`).
+
+  In DIMACS, literals are non-zero integers, with negative numbers variables with an optional negation.
+  We represent them as integers, with the invariant that they are non-zero.
+-/
+def ILit := { i : Int // i ≠ 0 }
+  deriving DecidableEq, Repr
+
+namespace IVar
+
+/-! # index -/
+
+/--
+  Converts an `IVar` into a 0-indexed `Nat`.
+
+  DIMACS variables are 1-indexed, but arrays are 0-indexed,
+  so `index` subtracts one and does the coercion.
+-/
+@[inline, always_inline]
+def index (v : IVar) : Nat := v.val - 1
+
+/-- Converts a 0-indexed `Nat` into an `IVar`.  -/
+@[inline, always_inline]
+def ofIndex (n : Nat) : IVar := ⟨n + 1, by omega⟩
+
+@[simp]
+theorem ofIndex_inj (n m : Nat) : ofIndex n = ofIndex m ↔ n = m := by
+  simp [ofIndex]
+  constructor
+  · rintro ⟨⟩; rfl
+  · rintro rfl; rfl
+
+instance instInhabited : Inhabited IVar := ⟨⟨1, by decide⟩⟩
+
+def toString : IVar → String
+  | ⟨n, _⟩ => s!"{n}"
+
+instance instToString : ToString IVar where
+  toString := toString
+
+instance instHashable : Hashable IVar where
+  hash v := hash v.val
+
+instance instOrd : Ord IVar where
+  compare a b := compare a.val b.val
+
+instance instLT : LT IVar where
+  lt a b := a.val < b.val
+
+theorem lt_def (a b : IVar) : (a < b) = (a.val < b.val) := rfl
+
+@[simp] theorem lt_ofIndex (a b : Nat) : ofIndex a < ofIndex b ↔ a < b := by simp [ofIndex, lt_def]
+
+instance instLE : LE IVar where
+  le a b := a.val ≤ b.val
+
+theorem le_def (a b : IVar) : (a ≤ b) = (a.val ≤ b.val) := rfl
+
+@[simp] theorem le_refl (a : IVar) : a ≤ a := Nat.le_refl _
+@[simp] theorem le_ofIndex (a b : Nat) : ofIndex a ≤ ofIndex b ↔ a ≤ b := by simp [ofIndex, le_def]
+
+instance : HAdd IVar Nat IVar where
+  hAdd v off := ⟨v.val + off, by have := v.property; omega⟩
+
+@[simp] theorem val_addNat (v : IVar) (x : Nat) : (v + x).val = v.val + x := rfl
+@[simp] theorem index_addNat (v : IVar) (x : Nat) : (v + x).index = v.index + x := by
+  have := v.property
+  simp [index]
+  omega
+
+theorem add_lt_of_pos (pos : 0 < x) (v : IVar) : v < v + x := by
+  rw [IVar.lt_def]; simp; omega
+
+@[simp] theorem add_lt_add_left (v : IVar) (x y : Nat) : v + x < v + y ↔ x < y := by
+  rw [IVar.lt_def]; simp
+
+protected def max : IVar → IVar → IVar
+  | ⟨v₁, _⟩, ⟨v₂, _⟩ => ⟨max v₁ v₂, by
+      have := Nat.le_max_left v₁ v₂
+      have := Nat.le_max_right v₁ v₂
+      omega
+    ⟩
+
+def toPosILit : IVar → ILit
+  | ⟨n, hn⟩ => ⟨Int.ofNat n, by exact Int.natAbs_pos.mp hn⟩
+
+def toNegILit : IVar → ILit
+  | ⟨n, hn⟩ => ⟨-Int.ofNat n, by
+    intro h_con
+    rw [Int.neg_eq_zero] at h_con
+    revert h_con
+    exact Int.natAbs_pos.mp hn⟩
+
+instance instCoeIVar : Coe IVar ILit where
+  coe v := toPosILit v
+
+
+end IVar
+
+--------------------------------------------------------------------------------
+
+namespace ILit
+
+instance instInhabited : Inhabited ILit := ⟨1, by decide⟩
+
+instance instHashable : Hashable ILit where
+  hash v := hash v.val
+
+instance instOrd : Ord ILit where
+  compare a b := compare a.val b.val
+
+instance instCoeInt : Coe ILit Int where
+  coe v := v.val
+
+def toString : ILit → String
+  | ⟨l, _⟩ => s!"{l}"
+
+instance instToString : ToString ILit where
+  toString := toString
+
+def toIVar : ILit → IVar
+  | ⟨l, hl⟩ => ⟨l.natAbs, Int.natAbs_pos.mpr hl⟩
+
+instance instCoeToIVar : Coe ILit IVar where
+  coe v := toIVar v
+
+def ofIVar : IVar → ILit
+  | ⟨n, hn⟩ => ⟨Int.ofNat n, by exact Int.natAbs_pos.mp hn⟩
+
+instance instCoeOfIVar : Coe IVar ILit where
+  coe v := ofIVar v
+
+instance instOfNat : OfNat ILit (n+1) := ⟨n+1, by omega⟩
+
+def toNat : ILit → Nat
+  | ⟨l, _⟩ => l.natAbs
+
+/-- Returns `true` iff the literal is positive. -/
+protected def polarity : ILit → Bool
+  | ⟨l, _⟩ => l > 0
+
+def negate : ILit → ILit
+  | ⟨l, _⟩ => ⟨-l, by
+    intro h
+    have := Int.neg_eq_zero.mp h
+    contradiction⟩
+
+instance instLitVar : LitVar ILit IVar where
+  negate l := ⟨-l.val, Int.neg_ne_zero.mpr l.property⟩
+  mkPos x := ⟨Int.ofNat x.val, by cases x; simp; omega⟩
+  mkNeg x := ⟨-Int.ofNat x.val, by cases x; simp; omega⟩
+  toVar l := ⟨Int.natAbs l.val, Int.natAbs_pos.mpr l.property⟩
+  polarity l := (0 : Int) < l.val
+
+instance instNeg : Neg ILit where
+  neg := LitVar.negate
+
+open LitVar in
+theorem polarity_eq {l₁ l₂ : ILit} :
+    polarity l₁ = polarity l₂ ↔ ((0 : Int) < l₁.val ↔ (0 : Int) < l₂.val) := by
+  simp [polarity]
+
+open LitVar in
+instance instLawfulLitVar : LawfulLitVar ILit IVar where
+  toVar_negate l := by
+    apply Subtype.ext
+    apply Int.natAbs_neg
+  toVar_mkPos x :=
+    Subtype.ext (Int.natAbs_ofNat x.val)
+  toVar_mkNeg x := by
+    apply Subtype.ext
+    simp [toVar, mkNeg]
+  polarity_negate l := by
+    rw [Bool.eq_bnot, polarity_eq]
+    intro hEq
+    exact l.property (Int.eq_zero_of_lt_neg_iff_lt _ hEq)
+  polarity_mkPos l := by
+    cases l
+    simp [polarity, mkPos]
+    assumption
+  polarity_mkNeg l := by
+    cases l
+    simp [polarity, mkNeg]
+    omega
+  ext l₁ l₂ := by
+    /- Strip type alias. -/
+    suffices ∀ {l₁ l₂ : Int}, l₁.natAbs = l₂.natAbs → (0 < l₁ ↔ 0 < l₂) → l₁ = l₂ by
+      intro h₁ h₂
+      apply Subtype.ext
+      apply this
+      . cases l₁; cases l₂
+        simp [toVar] at h₁
+        injection h₁
+      . exact polarity_eq.mp h₂
+    intro l₁ l₂ h₁ h₂
+    cases Int.natAbs_eq_natAbs_iff.mp h₁
+    . assumption
+    next h =>
+      rw [h] at h₂
+      have : l₂ = 0 := Int.eq_zero_of_lt_neg_iff_lt l₂ h₂
+      simp [this, h]
+
+/-! # index -/
+
+/--
+  Converts an `ILit` into a 0-indexed `Nat`.
+
+  DIMACS literals are 1-indexed (ignoring sign), but arrays are 0-indexed,
+  so `index` subtracts one and does the coercion.
+-/
+@[inline, always_inline]
+def index (l : ILit) : Nat := l.val.natAbs - 1
+
+/-- Converts a 0-indexed `Nat` into an `ILit`. -/
+@[inline, always_inline]
+def ofIndex (n : Nat) : ILit := ⟨n + 1, by omega⟩
+
+end ILit
+
+--------------------------------------------------------------------------------
+
+abbrev IClause := Clause ILit
+abbrev ICnf := Cnf ILit
+abbrev ICube := Cube ILit
+
+namespace IClause
+
+/--
+  Finds the maximum DIMACS variable in a clause.
+  If the clause is empty, then 0 is returned.
+-/
+def maxVar (C : IClause) : Nat :=
+  Array.map ILit.toNat C |> Array.foldl max 0
+
+end IClause
+
+namespace ICnf
+/--
+  Finds the maximum DIMACS variable in the CNF.
+  If there are no variables in the formula, then 0 is returned.
+-/
+def maxVar (F : ICnf) : Nat :=
+  Array.map IClause.maxVar F |> Array.foldl max 0
+
+end ICnf
+
+end Trestle
