Trestle/Data/LitVar/Basic.lean
@@ -1,0 +1,270 @@
+/-
+Copyright (c) 2025 The Trestle Contributors.
+Released under the Apache License v2.0; see LICENSE for full text.
+-/
+
+import Trestle.Upstream.ToStd
+import Trestle.Upstream.ToMathlib
+import Trestle.Data.LitVar.Defs
+import Trestle.Model.Subst
+
+/-!
+
+  Basic theorems about literals and variables.
+
+-/
+
+namespace Trestle
+
+open Model
+
+namespace LitVar
+
+variable {L : Type u} {ν : Type v} [LitVar L ν]
+
+def toPropForm (l : L) : PropForm ν :=
+  if polarity l then .var (toVar l) else .neg (.var $ toVar l)
+
+instance : CoeHead L (PropForm ν) := ⟨toPropForm⟩
+
+def toPropFun (l : L) : PropFun ν :=
+  if polarity l then .var (toVar l) else (.var $ toVar l)ᶜ
+
+instance : CoeHead L (PropFun ν) := ⟨toPropFun⟩
+
+open PropFun in
+theorem satisfies_iff {τ : PropAssignment ν} {l : L} :
+    τ ⊨ toPropFun l ↔ τ (toVar l) = polarity l := by
+  dsimp [toPropFun, polarity]
+  aesop
+
+-- Some theorems can be proven on `LitVar`s, without the `Lawful` laws.
+
+@[simp]
+theorem mk_toPropForm (l : L) : ⟦toPropForm l⟧ = toPropFun l := by
+  dsimp [toPropForm, toPropFun]
+  cases polarity l <;> simp
+
+@[simp]
+theorem vars_toPropForm [DecidableEq ν] (l : L) : (toPropForm l).vars = {toVar l} := by
+  dsimp [toPropForm]
+  cases polarity l <;> simp [PropForm.vars]
+
+@[simp]
+theorem semVars_toPropFun [DecidableEq ν] (l : L) : (toPropFun l).semVars = {toVar l} := by
+  dsimp [toPropFun]
+  cases polarity l <;> simp
+
+-- The rest of the theorems need the laws
+
+variable [LawfulLitVar L ν]
+
+open LawfulLitVar
+
+@[simp] theorem var_mkLit (x : ν) (p : Bool) : toVar (mkLit L x p) = x := by
+  dsimp [mkLit]; split <;> simp
+@[simp] theorem polarity_mkLit (x : ν) (p : Bool) : polarity (mkLit L x p) = p := by
+  dsimp [mkLit]; split <;> simp_all
+
+@[simp] theorem eta (l : L) : mkLit L (toVar l) (polarity l) = l := by
+  ext <;> simp
+@[simp] theorem eta_neg (l : L) : mkLit L (toVar l) (!polarity l) = -l := by
+  ext <;> simp
+
+theorem mkPos_or_mkNeg (l : L) : l = mkPos (toVar l) ∨ l = mkNeg (toVar l) := by
+  rw [← eta l]
+  cases polarity l
+  . apply Or.inr
+    simp [mkLit]
+  . apply Or.inl
+    simp [mkLit]
+
+-- CC: For better `rcases (... rfl)` patterns
+theorem exists_mkPos_or_mkNeg (l : L) : ∃ v, l = mkPos v ∨ l = mkNeg v := by
+  use toVar l
+  rcases mkPos_or_mkNeg l with (h | h)
+  · exact Or.inl h
+  · exact Or.inr h
+
+@[simp]
+theorem mkPos_ne_mkNeg {v₁ v₂ : ν} : mkPos (L := L) v₁ ≠ mkNeg (L := L) v₂ := by
+  intro h_con
+  have := LawfulLitVar.ext_iff.mp h_con
+  simp at this
+
+@[simp]
+theorem mkNeg_ne_mkPos {v₁ v₂ : ν} : mkNeg (L := L) v₁ ≠ mkPos (L := L) v₂ :=
+  Ne.symm (@mkPos_ne_mkNeg _ _ _ _ v₂ v₁)
+
+-- CC: Could also use `Function.Injective`
+@[simp]
+theorem mkPos_inj {x y : ν} : mkPos (L := L) x = mkPos (L := L) y ↔ x = y := by
+  constructor
+  · intro h
+    rcases LawfulLitVar.ext_iff.mp h with ⟨h, _⟩
+    simp at h
+    exact h
+  · rintro rfl
+    rfl
+
+@[simp]
+theorem mkNeg_inj {x y : ν} : mkNeg (L := L) x = mkNeg (L := L) y ↔ x = y := by
+  constructor
+  · intro h
+    rcases LawfulLitVar.ext_iff.mp h with ⟨h, _⟩
+    simp at h
+    exact h
+  · rintro rfl
+    rfl
+
+@[simp] theorem toPropForm_mkPos (x : ν) : toPropForm (mkPos (L := L) x) = .var x := by
+  simp [toPropForm]
+@[simp] theorem toPropForm_mkNeg (x : ν) : toPropForm (mkNeg (L := L) x) = .neg (.var x) := by
+  simp [toPropForm]
+
+@[simp] theorem toPropFun_mkPos (x : ν) : toPropFun (mkPos (L := L) x) = .var x := by
+  simp [toPropFun]
+@[simp] theorem toPropFun_mkNeg (x : ν) : toPropFun (mkNeg (L := L) x) = (.var x)ᶜ := by
+  simp [toPropFun]
+@[simp] theorem toPropFun_mkLit_true : toPropFun (mkLit L v true) = .var v := by
+  simp [toPropFun]
+@[simp] theorem toPropFun_mkLit_false : toPropFun (mkLit L v false) = (.var v)ᶜ := by
+  simp [toPropFun]
+@[simp] theorem toPropFun_neg (l : L) : toPropFun (-l) = (toPropFun l)ᶜ := by
+  dsimp [toPropFun]
+  aesop
+
+-- CC: This theorem already exists in the `LawfulLitVar` namespace
+--     due to `attribute [ext]`
+theorem ext_iff (l1 l2 : L) : l1 = l2 ↔ toVar l1 = toVar l2 ∧ polarity l1 = polarity l2 := by
+  constructor
+  · rintro rfl; simp
+  · aesop
+
+@[simp] theorem neg_eq_neg (l1 l2 : L) : -l1 = -l2 ↔ l1 = l2 := by
+  constructor
+  · rw [ext_iff, ext_iff (L := L)]; simp
+  · rintro rfl; rfl
+
+@[simp] theorem neg_neg (l : L) : - (- l) = l := by
+  rw [ext_iff]; simp
+
+@[simp] theorem neg_mkPos (x : ν) : - (mkPos (L := L) x) = mkNeg x := by
+  rw [ext_iff]; simp
+
+@[simp] theorem neg_mkNeg (x : ν) : - (mkNeg (L := L) x) = mkPos x := by
+  rw [ext_iff]; simp
+
+-- CC: Have a simp attribute here?
+theorem toVar_eq_iff {l₁ l₂ : L} : toVar l₁ = toVar l₂ ↔ (l₁ = l₂ ∨ l₁ = -l₂) := by
+  rcases exists_mkPos_or_mkNeg l₁ with ⟨v₁, (rfl | rfl)⟩
+  <;> rcases exists_mkPos_or_mkNeg l₂ with ⟨v₂, (rfl | rfl)⟩
+  <;> simp
+
+theorem toVar_eq_iff' {l₁ l₂ : L} : toVar l₁ = toVar l₂ ↔ (l₁ = l₂ ∨ -l₁ = l₂) := by
+  rcases exists_mkPos_or_mkNeg l₁ with ⟨v₁, (rfl | rfl)⟩
+  <;> rcases exists_mkPos_or_mkNeg l₂ with ⟨v₂, (rfl | rfl)⟩
+  <;> simp
+
+open PropFun
+
+theorem satisfies_neg {τ : PropAssignment ν} {l : L} :
+    τ ⊨ toPropFun (-l) ↔ τ ⊭ toPropFun l := by
+  simp [satisfies_iff]
+
+omit [LawfulLitVar L ν] in
+theorem satisfies_set [DecidableEq ν] (τ : PropAssignment ν) (l : L) :
+    τ.set (toVar l) (polarity l) ⊨ toPropFun l := by
+  simp [satisfies_iff, τ.set_get]
+
+theorem eq_of_flip [DecidableEq ν] {τ : PropAssignment ν} {l : L} {x : ν} {p : Bool} :
+    τ ⊭ toPropFun l → τ.set x p ⊨ toPropFun l → l = mkLit L x p := by
+  simp only [satisfies_iff]
+  intro h hSet
+  by_cases hEq : x = toVar l
+  . rw [hEq, τ.set_get] at hSet
+    simp [hSet, hEq]
+  . exfalso; exact h (τ.set_get_of_ne p hEq ▸ hSet)
+
+theorem eq_of_flip' [DecidableEq ν] {τ : PropAssignment ν} {l : L} {x : ν} {p : Bool} :
+    τ ⊨ toPropFun l → τ.set x p ⊭ toPropFun l → l = mkLit L x !p := by
+  simp only [satisfies_iff]
+  intro h hSet
+  by_cases hEq : x = toVar l
+  . rw [hEq, τ.set_get] at hSet
+    have : (!p) = polarity l := by
+      simp [Bool.eq_bnot, hSet]
+    simp [hEq, this]
+  . exfalso; exact hSet (τ.set_get_of_ne p hEq ▸ h)
+
+theorem toPropFun.inj [DecidableEq ν] : (toPropFun (L := L)).Injective := by
+  intro l₁ l₂ h; simp [toPropFun] at h
+  split_ifs at h
+  · rename_i h₁ h₂
+    rw [var_eq_var] at h
+    apply LawfulLitVar.ext _ _ h
+    rw [h₁, h₂]
+  · simp only [var_ne_var_compl] at h
+  · simp only [var_compl_ne_var] at h
+  · rename_i h₁ h₂
+    simp only [Bool.not_eq_true] at h₁ h₂
+    simp only [compl_inj_iff, var_eq_var] at h
+    apply LawfulLitVar.ext _ _ h
+    rw [h₁, h₂]
+
+/-! #### map -/
+
+@[simp]
+theorem satisfies_map [LitVar L V] [LitVar L' V']
+    [LawfulLitVar L' V'] (f : V → V') (l : L) (τ : PropAssignment V')
+  : τ ⊨ LitVar.toPropFun (LitVar.map f l : L') ↔ τ.map f ⊨ LitVar.toPropFun l
+  := by
+  simp [map, toPropFun]
+  split <;> simp
+
+@[simp]
+theorem toPropFun_map [LitVar L V] [LitVar L' V'] [LawfulLitVar L' V'] (f : V → V') (l : L)
+    : LitVar.toPropFun (LitVar.map f l : L') = (LitVar.toPropFun l).map f := by
+  ext τ; simp
+
+
+/-! #### Sums as valid literals -/
+
+section
+variable [LitVar L1 V1] [LitVar L2 V2]
+
+instance [LawfulLitVar L1 V1] [LawfulLitVar L2 V2]
+    : LawfulLitVar (L1 ⊕ L2) (V1 ⊕ V2) where
+  toVar_mkPos     := by rintro (_ | _) <;> simp [toVar, mkPos]
+  toVar_mkNeg     := by rintro (_ | _) <;> simp [toVar, mkNeg]
+  toVar_negate    := by rintro (_ | _) <;> simp_rw [Neg.neg, negate] <;> simp [toVar]
+  polarity_mkPos  := by rintro (_ | _) <;> simp [polarity, mkPos]
+  polarity_mkNeg  := by rintro (_ | _) <;> simp [polarity, mkNeg]
+  polarity_negate := by rintro (_ | _) <;> simp_rw [Neg.neg, negate] <;> simp [polarity]
+  ext := by
+    rintro (l₁ | l₁) (l₂ | l₂)
+    <;> rcases mkPos_or_mkNeg l₁ with (h₁ | h₁)
+    <;> rcases mkPos_or_mkNeg l₂ with (h₂ | h₂)
+    all_goals (
+      rw [h₁, h₂]
+      simp [toVar, polarity]
+      try intro h
+      try rw [h]
+    )
+
+@[simp] theorem polarity_inl (l : L1)
+  : polarity (L := L1 ⊕ L2) (ν := V1 ⊕ V2) (Sum.inl l) = polarity l := rfl
+
+@[simp] theorem polarity_inr (l : L2)
+  : polarity (L := L1 ⊕ L2) (ν := V1 ⊕ V2) (Sum.inr l) = polarity l := rfl
+
+@[simp] theorem toVar_inl (l : L1)
+  : toVar (L := L1 ⊕ L2) (ν := V1 ⊕ V2) (Sum.inl l) = .inl (toVar l) := rfl
+
+@[simp] theorem toVar_inr (l : L2)
+  : toVar (L := L1 ⊕ L2) (ν := V1 ⊕ V2) (Sum.inr l) = .inr (toVar l) := rfl
+end
+
+end LitVar
+
+end Trestle
