Trestle/Data/LitVar/Defs.lean
@@ -1,0 +1,79 @@
+/-
+Copyright (c) 2025 The Trestle Contributors.
+Released under the Apache License v2.0; see LICENSE for full text.
+-/
+
+namespace Trestle
+
+/-! ### Literals -/
+
+/-- The type `L` is a representation of literals over variables of type `ν`. -/
+@[specialize]
+class LitVar (L : Type u) (ν : outParam $ Type v) where
+  negate : L → L
+  mkPos : ν → L
+  mkNeg : ν → L := fun x => negate (mkPos x)
+  toVar : L → ν
+  /-- true if positive -/
+  polarity : L → Bool
+  -- TODO: ν moreover needs to biject with PNat (perhaps in a separate typeclass)
+  -- so that we can use variable names as array indices
+
+namespace LitVar
+
+def mkLit (L : Type u) {ν : Type v} [LitVar L ν] (x : ν) (p : Bool) : L :=
+  if p then mkPos x else mkNeg x
+
+def map [LitVar L V] [LitVar L' V'] (f : V → V') (l : L) : L' :=
+  LitVar.mkLit _ (f (LitVar.toVar l)) (LitVar.polarity l)
+
+variable {L : Type u} {ν : Type v} [LitVar L ν]
+
+-- controversial maybe?
+instance : Coe ν L :=
+  ⟨mkPos⟩
+
+instance : Neg L :=
+  ⟨negate⟩
+
+@[simp] theorem negate_eq (l : L) : negate l = -l := rfl
+
+instance [ToString ν] : ToString L where
+  toString l := if polarity l then s!"{toVar l}" else s!"-{toVar l}"
+
+end LitVar
+
+/-! ### Lawful literals -/
+
+-- TODO: see if a shorter list of axioms implies this one
+open LitVar in
+class LawfulLitVar (L : Type u) (ν : outParam (Type v)) [LitVar L ν] where
+  toVar_negate (l : L) : toVar (-l) = toVar l
+  toVar_mkPos (x : ν) : toVar (mkPos (L := L) x) = x
+  toVar_mkNeg (x : ν) : toVar (mkNeg (L := L) x) = x
+  polarity_negate (l : L) : polarity (-l) = !polarity l
+  polarity_mkPos (x : ν) : polarity (mkPos (L := L) x) = true
+  polarity_mkNeg (x : ν) : polarity (mkNeg (L := L) x) = false
+  protected ext (l₁ l₂ : L) : toVar l₁ = toVar l₂ → polarity l₁ = polarity l₂ → l₁ = l₂
+
+open LawfulLitVar in
+attribute [simp] toVar_negate toVar_mkPos toVar_mkNeg polarity_negate polarity_mkPos polarity_mkNeg
+
+open LawfulLitVar in
+attribute [ext] LawfulLitVar.ext
+
+
+/-! #### Sums as valid literals -/
+
+namespace LitVar
+
+instance [LitVar L1 V1] [LitVar L2 V2] : LitVar (L1 ⊕ L2) (V1 ⊕ V2) where
+  mkPos := Sum.map (LitVar.mkPos) (LitVar.mkPos)
+  mkNeg := Sum.map (LitVar.mkNeg) (LitVar.mkNeg)
+  toVar := Sum.map (LitVar.toVar) (LitVar.toVar)
+  polarity := fun | .inl l => LitVar.polarity l | .inr l => LitVar.polarity l
+  negate := Sum.map (LitVar.negate) (LitVar.negate)
+
+end LitVar
+
+end Trestle
