Trestle/Encode/Cardinality.lean
@@ -1,2 +1,3 @@
+import Trestle.Encode.Cardinality.AMO
+import Trestle.Encode.Cardinality.GeneralEncs
 import Trestle.Encode.Cardinality.Defs
-import Trestle.Encode.Cardinality.Encs
